nola/lrust/heap.v
@@ -148,7 +148,8 @@ Section heap.
 
   Lemma heap_pointsto_agree l q1 q2 v1 v2 : l ↦{q1} v1 ∗ l ↦{q2} v2 ⊢ ⌜v1 = v2⌝.
   Proof.
-    rewrite heap_pointsto_eq -own_op -auth_frag_op own_valid discrete_valid.
+    rewrite heap_pointsto_eq -own_op -auth_frag_op own_valid
+      internal_cmra_valid_discrete.
     eapply pure_elim; [done|]=> /auth_frag_valid /=.
     rewrite singleton_op -pair_op singleton_valid=> -[? /to_agree_op_inv_L->]; eauto.
   Qed.
